Core/Examples/Boolean.lean
@@ -62,7 +62,6 @@ def eqBool : Term := λ[ gt#"Bool" ] λ[ gt#"Bool" ]
 
 #guard Term.infer_type BoolCtx [] [] eqBool == some (gt#"Bool" -:> (gt#"Bool" -:> gt#"Bool"))
 
-
 def EqBoolCtx : GlobalEnv := [
   -- instance (==)[t] i
   --    If EqBool[t] t~Bool ← i
@@ -89,24 +88,30 @@ def EqBoolCtx : GlobalEnv := [
 
 
 #guard EqBoolCtx.wf_globals  == some ()
+
 #eval ((d#"eqBool" • TrueCtor) • TrueCtor).eval_loop EqBoolCtx
 #eval ((d#"eqBool" • TrueCtor) • FalseCtor).eval_loop EqBoolCtx
 
 def iBool : Term := inst! "EqBool" #𝓋[ gt#"Bool" ] (Vec.to #𝓋[ refl! gt#"Bool"])
-#eval! iBool.infer_type EqBoolCtx [] []
+#guard iBool.infer_type EqBoolCtx [] [] == some (gt#"Eq" • gt#"Bool")
+
+-- #eval get_instance "EqBool" ((#𝓋[ iBool ])) EqBoolCtx
 
 def t1 : Term := ((openm! "eq" #𝓋[ gt#"Bool" ] (Vec.to (#𝓋[ iBool ]))) • TrueCtor) • FalseCtor
-#eval! t1.infer_type EqBoolCtx [] []
+#guard t1.infer_type EqBoolCtx [] [] == some (gt#"Bool")
 -- def t2 : Term := (g#"eq" •[ gt#"Bool" ]  • (g#"EqBool" •[  gt#"Bool" ] • refl! gt#"Bool") • g#"True") • g#"True"
 
-#eval! t1.eval_loop EqBoolCtx
+#eval t1.eval_loop EqBoolCtx
 
 -- def ctx' := List.drop 1 EqBoolCtx
 -- #eval! (Λ[★] λ[(t#0 ~[★]~ gt#"Bool")] λ[t#0] λ[t#0]
 --              (((d#"eqBool" • (.cast t#0 #2 #1)) • (.cast t#0 #2 #0)))).infer_type EqBoolCtx [] []
 
 def t2 : Term := ((openm! "eq" #𝓋[ gt#"Bool" ] (Vec.to (#𝓋[ iBool ]))) • TrueCtor) • TrueCtor
-#eval! t2.eval_loop EqBoolCtx
+#eval t2.eval_loop EqBoolCtx
+
+def t3 : Term := ((openm! "eq" #𝓋[ gt#"Bool" ] (Vec.to (#𝓋[ iBool ]))) • TrueCtor) • FalseCtor
+#eval t3.eval_loop EqBoolCtx
 
 
 end Core.Examples
